examples/MemAtomic.v
@@ -126,23 +126,11 @@ Section MemAtomicWoQ.
       <<== (memAtomic addrSize lgDataBytes n).
   Proof.
     unfold memAtomic, memAtomicWoQ.
-    ketrans; [rewrite SemFacts.idElementwiseId; apply traceRefines_assoc_2|].
-
+    krewrite assoc left.
     kmodular_sim_l.
-    - knodup_regs.
-    - knodup_regs.
-    - knodup_regs.
-    - kdisj_regs.
-    - kdisj_regs.
-    - split.
-      + apply duplicate_regs_ConcatMod_2; [kequiv|kequiv|kvr|kvr| |]; auto.
-      + apply duplicate_regs_ConcatMod_1; [kequiv|kequiv|kvr|kvr| |]; auto.
-    - split.
-      + apply duplicate_rules_ConcatMod_2; [kequiv|kequiv|kvr|kvr| |]; auto.
-      + apply duplicate_rules_ConcatMod_1; [kequiv|kequiv|kvr|kvr| |]; auto.
-    - split.
-      + apply duplicate_defs_ConcatMod_2; [kequiv|kequiv|kvr|kvr| |]; auto.
-      + apply duplicate_defs_ConcatMod_1; [kequiv|kequiv|kvr|kvr| |]; auto.
+    - apply duplicate_regs_ConcatMod; [kequiv|kequiv|kvr|kvr| |]; auto.
+    - apply duplicate_rules_ConcatMod; [kequiv|kequiv|kvr|kvr| |]; auto.
+    - apply duplicate_defs_ConcatMod; [kequiv|kequiv|kvr|kvr| |]; auto.
   Qed.
 
 End MemAtomicWoQ.
